Prove type preservation of whole-program transform

fiat2/src/fiat2/IndexTransf2.v
@@ -1,5 +1,5 @@
 Require Import fiat2.Language fiat2.Interpret fiat2.Value fiat2.TypeSystem fiat2.TypeSound fiat2.IndexInterface2
-  fiat2.Utils fiat2.TransfSound fiat2.Substitute.
+  fiat2.Utils fiat2.TransfSound fiat2.Substitute fiat2.TransfUtils.
 Require Import coqutil.Map.Interface coqutil.Word.Interface coqutil.Datatypes.Result.
 Require Import List String ZArith Sorted Permutation.
 Import ListNotations.
@@ -21,167 +21,314 @@ Proof.
 Qed.
 
 Section compo_idx.
-  Section WithMap.
+  Context {tenv : map.map string type} {tenv_ok : map.ok tenv}.
+  Context {width: Z} {word: word.word width} {word_ok: word.ok word}.
+  Notation value := (value (width:=width)).
+  Context {locals : map.map string value} {locals_ok : map.ok locals}.
+
+  Context {idxs : list (string * IndexInterface2.index * (value -> value -> Prop))}.
+  Context {idxs_ok : Forall (fun '(_, idx, idx_wf) => ok idx idx_wf) idxs}.
+  Context (H_tag_NoDup : NoDup (List.map fst (List.map fst idxs))).
+  Context (hole0 : string).
+  Context (H_holes_eq : Forall (fun '(_, idx, _) => @hole idx = hole0) idxs).
+
+  Definition compo_idx_ty (t : type) : type :=
+    TRecord (record_sort (List.map (fun '(tag, idx, _) => (tag, @idx_ty idx t)) idxs)).
+
+  Definition to_compo_idx : expr :=
+    ERecord (List.map (fun '(tag, idx, _) => (tag, @to_idx idx)) idxs).
+
+  Definition compo_idx_wf (v v' : value) : Prop :=
+    match v' with
+    | VRecord v' =>
+        Forall (fun '(tag, _, idx_wf) => idx_wf v (record_proj tag v')) idxs
+    | _ => False
+    end.
+
+  Definition compo_is_tbl_ty (t : type) : bool :=
+    forallb (fun '(tag, idx, _) => @is_tbl_ty idx t) idxs.
+
+  Lemma to_compo_idx_ty : forall (t : type),
+      type_wf t -> compo_is_tbl_ty t = true ->
+      type_of map.empty (map.put map.empty hole0 t) to_compo_idx (compo_idx_ty t).
+  Proof.
+    unfold compo_is_tbl_ty, to_compo_idx, compo_idx_ty.
+    intros. econstructor; eauto using Permuted_record_sort, StronglySorted_record_sort.
+    1:{ clear. induction idxs; cbn; auto.
+        do 2 case_match; cbn; congruence. }
+    1:{ induction idxs; auto. cbn in *.
+        repeat invert_Forall; invert_NoDup; rewrite Bool.andb_true_iff in *; intuition idtac.
+        constructor; auto.
+        do 2 case_match; cbn; subst. eapply (to_idx_ty (idx:=i)); eauto. }
+    1:{ revert H_tag_NoDup; clear; intros.
+        induction idxs; intros; cbn; auto using NoDup_nil.
+        cbn in *; invert_NoDup.
+        constructor; auto. do 2 case_match; cbn in *.
+        rewrite map_fst_map_triple; auto. }
+  Qed.
+
+  Lemma compo_idx_ty_wf : forall t : type,
+      type_wf t -> compo_is_tbl_ty t = true ->
+      type_wf (compo_idx_ty t).
+  Proof.
+    unfold compo_is_tbl_ty, compo_idx_ty; intros ? ? H.
+    eapply List.forallb_to_Forall with (P:=fun '(_, idx, _) => @is_tbl_ty idx t = true) in H.
+    2: intros; repeat case_match; auto.
+    constructor; auto using StronglySorted_record_sort.
+    1:{ eapply Permutation_NoDup.
+        1: apply Permutation_map, Permuted_record_sort.
+        induction idxs; cbn in *; auto.
+        repeat invert_Forall; invert_NoDup.
+        constructor; auto.
+        repeat case_match; cbn in *.
+        rewrite map_fst_map_triple; auto. }
+    1:{ rewrite Forall_map.
+        eapply Permutation_Forall.
+        1: apply Permuted_record_sort.
+        induction H; cbn in *; auto.
+        repeat invert_Forall; invert_NoDup.
+        constructor; repeat case_match; auto.
+        cbn; auto using idx_ty_wf. }
+  Qed.
+
+  Lemma NoDup_In_access_record : forall A (l : list (string * A)),
+      NoDup (List.map fst l) ->
+      forall s v, In (s, v) l ->
+                  access_record l s = Success v.
+  Proof.
+    intros * ? ? ? H_in; induction l; cbn in *.
+    1: intuition fail.
+    do 2 case_match; rewrite ?eqb_eq, ?eqb_neq in *; invert_NoDup.
+    1:{ subst. intuition idtac; try congruence.
+        apply in_map with (f:=fst) in H0;
+          cbn in *; intuition idtac. }
+    1:{ intuition idtac. congruence. }
+  Qed.
+
+  Lemma NoDup_Permutation_access_record : forall s A (l l' : list (string * A)),
+      NoDup (List.map fst l) ->
+      In s (List.map fst l) ->
+      Permutation l l' ->
+      access_record l s = access_record l' s.
+  Proof.
+    intros * H_NoDup H_in H_permu.
+    apply In_access_record in H_in. destruct_exists.
+    rewrite_l_to_r.
+    apply access_record_sound in H.
+    symmetry. apply NoDup_In_access_record.
+    1:{ eapply Permutation_NoDup.
+        1: apply Permutation_map; eauto.
+        assumption. }
+    1:{ eapply Permutation_in; eauto. }
+  Qed.
+
+  Lemma to_compo_idx_wf : forall (v : value) (t : type),
+      type_wf t -> compo_is_tbl_ty t = true ->
+      type_of_value v t ->
+      compo_idx_wf v (interp_expr map.empty (map.put map.empty hole0 v) to_compo_idx).
+  Proof.
+    intros.
+    unfold compo_idx_wf, compo_idx_ty, to_compo_idx, compo_is_tbl_ty, record_proj in *.
+    cbn [interp_expr].
+    rewrite Forall_forall; intros. do 2 case_match.
+    erewrite NoDup_Permutation_access_record.
+    4: apply Permutation_sym, Permuted_record_sort.
+    2:{ eapply Permutation_NoDup.
+        1: eapply Permutation_map, Permuted_record_sort.
+        rewrite fst_map_fst, map_fst_map_triple; auto. }
+    2:{ rewrite in_map_iff. eexists; intuition idtac.
+        2:{ eapply Permutation_in.
+            1: apply Permuted_record_sort.
+            rewrite in_map_iff. exists (s, to_idx).
+            intuition idtac.
+            rewrite in_map_iff; exists x.
+            subst; auto. }
+        reflexivity. }
+    eapply List.forallb_to_Forall with (P:=fun '(_, idx, _) => @is_tbl_ty idx t = true) in H0.
+    2: intros; repeat case_match; auto.
+    repeat apply_Forall_In. cbn in *.
+    apply to_idx_wf in H1; auto.
+    erewrite NoDup_In_access_record; eauto.
+    2:{ erewrite in_map_iff. exists (s, to_idx).
+        subst; intuition auto.
+        erewrite in_map_iff. exists (s, i, P); auto. }
+    rewrite fst_map_fst, map_fst_map_triple; auto.
+  Qed.
+
+  Instance compo_idx : IndexInterface2.index := IndexInterface2.mk hole0 to_compo_idx compo_idx_ty compo_is_tbl_ty.
+
+  Instance compo_idx_ok : IndexInterface2.ok compo_idx compo_idx_wf :=
+    IndexInterface2.Build_ok compo_idx compo_idx_wf compo_idx_ty_wf to_compo_idx_ty to_compo_idx_wf.
+End compo_idx.
+
+Section WithMap.
     Context {tenv : map.map string type} {tenv_ok : map.ok tenv}.
     Context {width: Z} {word: word.word width} {word_ok: word.ok word}.
     Notation value := (value (width:=width)).
     Context {locals : map.map string value} {locals_ok : map.ok locals}.
 
-    Context (idxs : list (string * IndexInterface2.index * (value -> value -> Prop))).
-    Context (idxs_ok : Forall (fun '(_, idx, idx_wf) => ok idx idx_wf) idxs).
-    Context (H_tag_NoDup : NoDup (List.map fst (List.map fst idxs))).
-    Context (hole0 : string).
-    Context (H_holes_eq : Forall (fun '(_, idx, _) => @hole idx = hole0) idxs).
+    Section WithIndex.
+      Context {idx : IndexInterface2.index} {idx_wf : value -> value -> Prop} {idx_ok : ok idx idx_wf}.
+      Context (id_tag aux_tag: string).
+      Context (H_tags_diff : id_tag <> aux_tag).
+      Context (tbl : string).
 
-    Definition compo_idx_ty (t : type) : type :=
-      TRecord (record_sort (List.map (fun '(tag, idx, _) => (tag, @idx_ty idx t)) idxs)).
+      Definition create_aux_write_head (free_vars : list string) (c : command) :=
+        match c with
+        | CAssign tbl' e =>
+            if String.eqb tbl tbl'
+            then CAssign tbl (ERecord [(id_tag, e); (aux_tag, substitute ((hole, e) :: nil) free_vars to_idx)])
+            else c
+        | _ => c
+        end.
 
-    Definition to_compo_idx : expr :=
-      ERecord (List.map (fun '(tag, idx, _) => (tag, @to_idx idx)) idxs).
+      Definition create_aux_read_head (e : expr) :=
+        match e with
+        | ELoc x => if String.eqb tbl x
+                    then (EAccess (ELoc tbl) id_tag)
+                    else e
+        | _ => e
+        end.
 
-    Definition compo_idx_wf (v v' : value) : Prop :=
-      match v' with
-      | VRecord v' =>
-          Forall (fun '(tag, _, idx_wf) => idx_wf v (record_proj tag v')) idxs
-      | _ => False
-      end.
+      Definition transf_to_idx' (free_vars : list string) (c : command) : command :=
+        fold_command_with_global tbl create_aux_write_head create_aux_read_head free_vars c.
 
-    Definition compo_is_tbl_ty (t : type) : bool :=
-      forallb (fun '(tag, idx, _) => @is_tbl_ty idx t) idxs.
+      Definition transf_to_idx (free_vars : list string) (c : command) : command :=
+        match c with
+        | CLetMut e tbl c =>
+            CLetMut (ERecord [(id_tag, e); (aux_tag, substitute ((hole, e) :: nil) free_vars to_idx)]) tbl
+              (transf_to_idx' free_vars c)
+        | _ => c
+        end.
 
-    Lemma to_compo_idx_ty : forall (t : type),
-        type_wf t -> compo_is_tbl_ty t = true ->
-        type_of map.empty (map.put map.empty hole0 t) to_compo_idx (compo_idx_ty t).
-    Proof.
-      unfold compo_is_tbl_ty, to_compo_idx, compo_idx_ty.
-      intros. econstructor; eauto using Permuted_record_sort, StronglySorted_record_sort.
-      1:{ clear. induction idxs; cbn; auto.
-          do 2 case_match; cbn; congruence. }
-      1:{ induction idxs; auto. cbn in *.
-          repeat invert_Forall; invert_NoDup; rewrite Bool.andb_true_iff in *; intuition idtac.
-          constructor; auto.
-          do 2 case_match; cbn; subst. eapply (to_idx_ty (idx:=i)); eauto. }
-      1:{ revert H_tag_NoDup; clear; intros.
-          induction idxs; intros; cbn; auto using NoDup_nil.
-          cbn in *; invert_NoDup.
-          constructor; auto. do 2 case_match; cbn in *.
-          rewrite map_fst_map_triple; auto. }
-    Qed.
+      Ltac apply_transf_to_idx_preserve_ty''_IH :=
+        lazymatch goal with IH: context[type_of _ _ ?e _ ] |- type_of _ _ ?e _ => apply IH end.
 
-    Lemma compo_idx_ty_wf : forall t : type,
-        type_wf t -> compo_is_tbl_ty t = true ->
-        type_wf (compo_idx_ty t).
-    Proof.
-      unfold compo_is_tbl_ty, compo_idx_ty; intros ? ? H.
-      eapply List.forallb_to_Forall with (P:=fun '(_, idx, _) => @is_tbl_ty idx t = true) in H.
-      2: intros; repeat case_match; auto.
-      constructor; auto using StronglySorted_record_sort.
-      1:{ eapply Permutation_NoDup.
-          1: apply Permutation_map, Permuted_record_sort.
-          induction idxs; cbn in *; auto.
-          repeat invert_Forall; invert_NoDup.
-          constructor; auto.
-          repeat case_match; cbn in *.
-          rewrite map_fst_map_triple; auto. }
-      1:{ rewrite Forall_map.
-          eapply Permutation_Forall.
-          1: apply Permuted_record_sort.
-          induction H; cbn in *; auto.
-          repeat invert_Forall; invert_NoDup.
-          constructor; repeat case_match; auto.
-          cbn; auto using idx_ty_wf. }
-    Qed.
+      Lemma transf_to_idx_preserve_ty'' : forall tbl_ty e Gstore Genv t,
+          tenv_wf Gstore -> tenv_wf Genv ->
+          map.get Gstore tbl = Some tbl_ty ->
+          is_tbl_ty tbl_ty = true ->
+          type_of Gstore Genv e t ->
+          type_of (map.put Gstore tbl
+                     (TRecord
+                        (record_sort
+                           [(id_tag, tbl_ty); (aux_tag, idx_ty tbl_ty)]))) Genv (fold_expr create_aux_read_head e) t.
+      Proof.
+        induction 5 using type_of_IH; simpl; intros.
+        all: try (econstructor; eauto; apply_transf_to_idx_preserve_ty''_IH; apply tenv_wf_step; eauto with fiat2_hints).
+        3: repeat apply tenv_wf_step; eauto with fiat2_hints.
+        1:{ case_match; rewrite ?eqb_eq, ?eqb_neq in *; subst.
+            1:{ repeat rewrite_l_to_r; do_injection.
+                repeat econstructor; try rewrite_map_get_put_goal; eauto.
+                apply NoDup_In_access_record.
+                1:{ eapply Permutation_NoDup.
+                    1: eapply Permutation_map; apply Permuted_record_sort.
+                    cbn; repeat constructor; intuition idtac.
+                    destruct_In; auto. }
+                eapply Permutation_in; [ apply Permuted_record_sort | ].
+                cbn; auto. }
+            constructor. rewrite_map_get_put_goal. }
+        1:{ econstructor; eauto.
+            1: rewrite fst_map_fst; assumption.
+            lazymatch goal with
+              H1: map fst _ = _, H2: Forall2 (type_of _ _) _ _,
+                  H3: Permutation _ _, H4: NoDup _ |- _ => clear H1 H2 H3 H4 end.
+            generalize dependent tl.
+            induction l; intros; simpl in *; invert_Forall2; auto.
+            case_match; simpl in *. constructor; auto.
+            destruct tl; simpl in *; try congruence. invert_cons.
+            apply IHl; auto. }
+      Qed.
 
-    Lemma NoDup_In_access_record : forall A (l : list (string * A)),
-        NoDup (List.map fst l) ->
-        forall s v, In (s, v) l ->
-        access_record l s = Success v.
-    Proof.
-      intros * ? ? ? H_in; induction l; cbn in *.
-      1: intuition fail.
-      do 2 case_match; rewrite ?eqb_eq, ?eqb_neq in *; invert_NoDup.
-      1:{ subst. intuition idtac; try congruence.
-          apply in_map with (f:=fst) in H0;
-            cbn in *; intuition idtac. }
-      1:{ intuition idtac. congruence. }
-    Qed.
+      Ltac use_transf_to_idx_preserve_ty'_IH :=
+        lazymatch goal with
+          IH: context[well_typed _ _ (transf_to_idx' _ ?c)] |- well_typed _ _ (transf_to_idx' _ ?c) =>
+            eapply IH; try reflexivity
+        end.
 
-    Lemma NoDup_Permutation_access_record : forall s A (l l' : list (string * A)),
-        NoDup (List.map fst l) ->
-        In s (List.map fst l) ->
-        Permutation l l' ->
-        access_record l s = access_record l' s.
-    Proof.
-      intros * H_NoDup H_in H_permu.
-      apply In_access_record in H_in. destruct_exists.
-      rewrite_l_to_r.
-      apply access_record_sound in H.
-      symmetry. apply NoDup_In_access_record.
-      1:{ eapply Permutation_NoDup.
-          1: apply Permutation_map; eauto.
-          assumption. }
-      1:{ eapply Permutation_in; eauto. }
-    Qed.
+      Lemma transf_to_idx_preserve_ty' : forall tbl_ty c (Gstore Gstore' Genv :tenv) free_vars,
+          tenv_wf Gstore -> tenv_wf Genv ->
+          map.get Gstore tbl = Some tbl_ty ->
+          is_tbl_ty tbl_ty = true ->
+          well_typed Gstore Genv c ->
+          incl (get_free_vars Genv) free_vars ->
+          Gstore' = map.put Gstore tbl
+                      (TRecord
+                         (record_sort
+                            [(id_tag, tbl_ty); (aux_tag, idx_ty tbl_ty)])) ->
+          well_typed Gstore' Genv (transf_to_idx' free_vars c).
+      Proof.
+        induction c; simpl; intros; try invert_well_typed; try now (constructor; auto).
+        1: econstructor; eauto using transf_to_idx_preserve_ty''.
+        1:{ econstructor; eauto using transf_to_idx_preserve_ty''.
+            use_transf_to_idx_preserve_ty'_IH; eauto with fiat2_hints.
+            eauto using incl_tran, incl_cons_step, get_free_vars_put. }
+        1:{ econstructor; eauto using transf_to_idx_preserve_ty''.
+            case_match; rewrite ?eqb_eq, ?eqb_neq in *; subst;
+              [ rewrite Properties.map.put_put_same in *; auto
+              | rewrite Properties.map.put_put_diff in *; auto;
+                use_transf_to_idx_preserve_ty'_IH; eauto with fiat2_hints ].
+            rewrite_map_get_put_goal. }
+        1:{ case_match; rewrite ?eqb_eq, ?eqb_neq in *; subst.
+            1:{ econstructor; [ rewrite_map_get_put_goal; eauto | ].
+                econstructor.
+                3: apply Permuted_record_sort.
+                1: reflexivity.
+                1:{ repeat constructor; cbn [snd].
+                    1:{ invert_well_typed.
+                        repeat rewrite_l_to_r; repeat (do_injection; clear_refl).
+                        eauto using transf_to_idx_preserve_ty''. }
+                    1:{ eapply substitute_preserve_ty with (Genv0:=map.put map.empty hole tbl_ty);
+                        eauto using idx_ty_wf with fiat2_hints.
+                        1:{ apply tenv_wf_step; auto. constructor; auto using StronglySorted_record_sort.
+                            1: eapply Permutation_NoDup;
+                            [ eapply Permutation_map, Permuted_record_sort
+                            | cbn; repeat constructor; intuition idtac;
+                              destruct_In; auto ].
+                            1:{ eapply Permutation_Forall;
+                                [ eapply Permutation_map, Permuted_record_sort | ].
+                                cbn. repeat constructor; eauto using idx_ty_wf. } }
+                1:{ eapply type_of_strengthen; eauto using to_idx_ty, map_incl_refl.
+                    apply map_incl_empty. }
+                1:{ unfold sub_wf. simpl; intros.
+                    case_match_string_eqb; rewrite_l_to_r; repeat do_injection;
+                      [ auto using transf_to_idx_preserve_ty''
+                      | rewrite map.get_empty in *; discriminate ]. } } }
+                1: cbn; repeat constructor; intuition idtac; destruct_In; auto.
+                1: apply StronglySorted_record_sort. }
+                1:{ econstructor; eauto using transf_to_idx_preserve_ty''.
+                    rewrite_map_get_put_goal; eauto. } }
+            1: constructor; eauto using transf_to_idx_preserve_ty''.
+        1:{ econstructor; eauto using transf_to_idx_preserve_ty''.
+            use_transf_to_idx_preserve_ty'_IH; eauto with fiat2_hints.
+            eauto using incl_tran, incl_cons_step, get_free_vars_put. }
+      Qed.
 
-    Lemma to_compo_idx_wf : forall (v : value) (t : type),
-      type_wf t -> compo_is_tbl_ty t = true ->
-      type_of_value v t ->
-      compo_idx_wf v (interp_expr map.empty (map.put map.empty hole0 v) to_compo_idx).
-    Proof.
-      intros.
-      unfold compo_idx_wf, compo_idx_ty, to_compo_idx, compo_is_tbl_ty, record_proj in *.
-      cbn [interp_expr].
-      rewrite Forall_forall; intros. do 2 case_match.
-      erewrite NoDup_Permutation_access_record.
-      4: apply Permutation_sym, Permuted_record_sort.
-      2:{ eapply Permutation_NoDup.
-          1: eapply Permutation_map, Permuted_record_sort.
-          rewrite fst_map_fst, map_fst_map_triple; auto. }
-      2:{ rewrite in_map_iff. eexists; intuition idtac.
-          2:{ eapply Permutation_in.
-              1: apply Permuted_record_sort.
-              rewrite in_map_iff. exists (s, to_idx).
-              intuition idtac.
-              rewrite in_map_iff; exists x.
-              subst; auto. }
-          reflexivity. }
-      eapply List.forallb_to_Forall with (P:=fun '(_, idx, _) => @is_tbl_ty idx t = true) in H0.
-      2: intros; repeat case_match; auto.
-      repeat apply_Forall_In. cbn in *.
-      apply to_idx_wf in H1; auto.
-      erewrite NoDup_In_access_record; eauto.
-      2:{ erewrite in_map_iff. exists (s, to_idx).
-          subst; intuition auto.
-          erewrite in_map_iff. exists (s, i, P); auto. }
-      rewrite fst_map_fst, map_fst_map_triple; auto.
-    Qed.
-
-    Instance compo_idx : IndexInterface2.index := IndexInterface2.mk hole0 to_compo_idx compo_idx_ty compo_is_tbl_ty.
-
-    Instance compo_idx_ok : IndexInterface2.ok compo_idx compo_idx_wf :=
-      IndexInterface2.Build_ok compo_idx compo_idx_wf compo_idx_ty_wf to_compo_idx_ty to_compo_idx_wf.
-  End WithMap.
-End compo_idx.
-
-Section WithTags.
-  Context (id_tag aux_tag: string).
-  Context (tbl : string).
-  Context (idx : IndexInterface2.index).
-
-  Definition create_aux_write_head (free_vars : list string) (c : command) :=
-    match c with
-    | CAssign tbl' e =>
-        if String.eqb tbl tbl'
-        then CAssign tbl (ERecord [(id_tag, e); (aux_tag, substitute ((@hole idx, e) :: nil) free_vars (@to_idx idx))])
-        else c
-    | _ => c
-    end.
-
-  Definition create_aux_read_head (e : expr) :=
-    match e with
-    | ELoc x => if String.eqb tbl x
-                then (EAccess (ELoc tbl) id_tag)
-                else e
-    | _ => e
-    end.
+      Lemma transf_to_idx_preserve_ty : forall tbl_ty e c free_vars Gstore Genv,
+          tenv_wf Gstore -> tenv_wf Genv ->
+          type_of Gstore Genv e tbl_ty ->
+          well_typed (map.put Gstore tbl tbl_ty) Genv c ->
+          is_tbl_ty tbl_ty = true ->
+          incl (get_free_vars Genv) free_vars ->
+          well_typed Gstore Genv (transf_to_idx free_vars (CLetMut e tbl c)).
+      Proof.
+        simpl; intros. subst. econstructor.
+        1:{ econstructor.
+            1: instantiate (1:=[(id_tag, tbl_ty); (aux_tag, idx_ty tbl_ty)]); reflexivity.
+            1:{ cbn; repeat constructor; auto.
+                eapply substitute_preserve_ty with (Genv0:=map.put map.empty hole tbl_ty); eauto using incl_refl with fiat2_hints.
+            1: eapply type_of_strengthen; [ apply to_idx_ty; eauto | apply map_incl_empty | apply map_incl_refl ].
+            1: eapply type_of__type_wf; [ | | eauto ]; auto.
+            1:{ unfold sub_wf. simpl; intros.
+                destruct_get_put_strings;
+                  [ do_injection; rewrite eqb_refl; auto
+                  | rewrite map.get_empty in *; discriminate ]. } }
+            1: eapply Permuted_record_sort.
+            1:{ cbn; repeat constructor; intuition auto. inversion H5; auto using in_nil. }
+            1: apply StronglySorted_record_sort. }
+        1:{ erewrite <- Properties.map.put_put_same.
+            eapply transf_to_idx_preserve_ty'; try reflexivity; eauto using incl_refl with fiat2_hints.
+            rewrite_map_get_put_goal; auto. }
+      Qed.
+    End WithIndex.
 End WithTags.
